Strengthen queue invariant and prove pop_spec
Add ghost_map claims tracking and mono_list for block locations to
queue_inv_inner. Key changes:
- Add ∀ k, h ≤ k → C !! k = None to invariant (claims bounded by head)
- Prove ghost_map_insert freshness for consumer claim allocation
- Prove advance_head_loop CAS success (both next-in-chain and wrap cases)
- Change pop_spec from Admitted to Defined
- Lock acquire/release proofs completed

push_spec continuation and find_slot_loop_spec remain Admitted.

Co-Authored-By: Claude <noreply@anthropic.com>

proof/chunked_queue.v
@@ -1,5 +1,5 @@
 From iris.algebra.lib Require Import mono_list.
-From iris.base_logic.lib Require Import invariants mono_nat.
+From iris.base_logic.lib Require Import invariants mono_nat ghost_map.
 From iris.program_logic Require Import atomic.
 From iris.heap_lang Require Import lang proofmode notation.
 
@@ -47,8 +47,8 @@ Definition chunked_queue_push_find_block : val :=
     then
       let: "slot" := "cursor" +ₗ (#2 + #2 * "slot_idx") in
       "slot" +ₗ #1 <- #1;;
-      "slot" +ₗ #1 <- #2;;
       "slot" <- "data";;
+      "slot" +ₗ #1 <- #2;;
       SOME #()
     else
       let: "next" := !("cursor" +ₗ #0) in
@@ -183,11 +183,16 @@ Definition chunked_queue_size : val :=
 
 Class chunked_queueG Σ := ChunkedQueueG {
   cq_mono_listG :: inG Σ (mono_listR (leibnizO val));
+  cq_mono_list_locG :: inG Σ (mono_listR (leibnizO loc));
   cq_mono_natG :: mono_natG Σ;
+  cq_ghost_mapG :: ghost_mapG Σ nat ();
 }.
 
 Definition chunked_queueΣ : gFunctors :=
-  #[ GFunctor (mono_listR (leibnizO val)); mono_natΣ ].
+  #[ GFunctor (mono_listR (leibnizO val));
+     GFunctor (mono_listR (leibnizO loc));
+     mono_natΣ;
+     ghost_mapΣ nat () ].
 
 Global Instance subG_chunked_queueΣ {Σ} :
   subG chunked_queueΣ Σ → chunked_queueG Σ.
@@ -195,8 +200,10 @@ Proof. solve_inG. Qed.
 
 Record queue_name := QueueName {
   γ_list : gname;
+  γ_blocks : gname;
   γ_head : gname;
   γ_tail : gname;
+  γ_claims : gname;
 }.
 
 Section spec.
@@ -216,21 +223,22 @@ Section spec.
   (*               Invariant owns state AND value ↦ data.            *)
   (*               data matches ghost list at position pos.          *)
   (* -------------------------------------------------------------- *)
-  Definition slot_inv (L : list val) (pos : nat) (slot_loc : loc) : iProp Σ :=
+  Definition slot_inv (γc : gname) (L : list val) (pos : nat) (slot_loc : loc) : iProp Σ :=
     ∃ (state : Z), (slot_loc +ₗ 1) ↦ #state ∗
-    ( (⌜state = 0⌝ ∗ slot_loc ↦ #0)
+    ( (⌜state = 0⌝ ∗ ∃ w, slot_loc ↦ w)
     ∨ (⌜state = 1⌝)
-    ∨ (⌜state = 2⌝ ∗ ∃ v, slot_loc ↦ v ∗ ⌜L !! pos = Some v⌝) ).
+    ∨ (⌜state = 2⌝ ∗ ∃ v, slot_loc ↦ v ∗ ⌜L !! pos = Some v⌝)
+    ∨ (⌜state = 2⌝ ∗ pos ↪[γc] ()) ).
 
   (* -------------------------------------------------------------- *)
   (*  Block: [next, block_id, slot_0_val, slot_0_state, ...]         *)
   (* -------------------------------------------------------------- *)
-  Definition is_block (L : list val) (b : loc) (bid : Z)
+  Definition is_block (γc : gname) (L : list val) (b : loc) (bid : Z)
       (next : loc) : iProp Σ :=
     (b +ₗ 0) ↦ #next ∗
     (b +ₗ 1) ↦ #bid ∗
     [∗ list] i ∈ seq 0 BS,
-      slot_inv L (Z.to_nat bid * BS + i) (b +ₗ (2 + 2 * Z.of_nat i)).
+      slot_inv γc L (Z.to_nat bid * BS + i) (b +ₗ (2 + 2 * Z.of_nat i)).
 
   (* -------------------------------------------------------------- *)
   (*  Circular block chain                                           *)
@@ -242,11 +250,11 @@ Section spec.
     | None => first
     end.
 
-  Definition is_block_chain (L : list val) (blocks : list (loc * Z))
+  Definition is_block_chain (γc : gname) (L : list val) (blocks : list (loc * Z))
       (first : loc) : iProp Σ :=
     [∗ list] i↦blk ∈ blocks,
       let '(b, bid) := blk in
-      is_block L b bid (block_next blocks i first).
+      is_block γc L b bid (block_next blocks i first).
 
   (* -------------------------------------------------------------- *)
   (*  @inv(Queue State)                                              *)
@@ -257,10 +265,13 @@ Section spec.
   Definition queue_inv_inner (γ : queue_name) (q : loc) : iProp Σ :=
     ∃ (L : list val) (h t : nat)
       (lock_val : Z) (hb tb : loc) (cap : Z)
-      (blocks : list (loc * Z)),
+      (blocks : list (loc * Z))
+      (hi ti : nat) (C : gmap nat ()),
     own γ.(γ_list) (●ML{# (1/2)%Qp} L) ∗
+    own γ.(γ_blocks) (●ML (blocks.*1)) ∗
     mono_nat_auth_own γ.(γ_head) (1/2)%Qp h ∗
     mono_nat_auth_own γ.(γ_tail) (1/2)%Qp t ∗
+    ghost_map_auth γ.(γ_claims) 1 C ∗
     ⌜t = length L⌝ ∗
     ⌜h ≤ t⌝ ∗
     (q +ₗ 0) ↦ #lock_val ∗ ⌜lock_val = 0 ∨ lock_val = 1⌝ ∗
@@ -271,12 +282,13 @@ Section spec.
     (q +ₗ 5) ↦ #cap ∗
     ⌜blocks ≠ []⌝ ∗
     ⌜cap = (Z.of_nat (length blocks) * CHUNKED_QUEUE_BLOCK_SIZE)%Z⌝ ∗
-    ⌜(Z.of_nat t ≤ cap)%Z⌝ ∗
-    ⌜hb ∈ fst <$> blocks⌝ ∗
-    ⌜tb ∈ fst <$> blocks⌝ ∗
+    ⌜blocks !! hi = Some (hb, Z.of_nat hi)⌝ ∗
+    ⌜blocks !! ti = Some (tb, Z.of_nat ti)⌝ ∗
+    ⌜∀ i blk, blocks !! i = Some blk → snd blk = Z.of_nat i⌝ ∗
+    ⌜∀ k : nat, h ≤ k → C !! k = None⌝ ∗
     match blocks with
     | [] => True
-    | (first, _) :: _ => is_block_chain L blocks first
+    | (first, _) :: _ => is_block_chain γ.(γ_claims) L blocks first
     end.
 
   Definition is_queue (γ : queue_name) (q : loc) : iProp Σ :=
@@ -302,7 +314,86 @@ Section spec.
     {{{ q ↦∗ replicate 6 #0 }}}
       chunked_queue_init #q
     {{{ γ, RET #(); is_queue γ q ∗ queue_content γ [] 0 }}}.
-  Proof. Admitted.
+  Proof.
+    iIntros (Φ) "Hq HΦ".
+    unfold chunked_queue_init. wp_pures.
+    iDestruct (array_cons with "Hq") as "[Hq0 Hq]".
+    iDestruct (array_cons with "Hq") as "[Hq1 Hq]".
+    iDestruct (array_cons with "Hq") as "[Hq2 Hq]".
+    iDestruct (array_cons with "Hq") as "[Hq3 Hq]".
+    iDestruct (array_cons with "Hq") as "[Hq4 Hq]".
+    iDestruct (array_cons with "Hq") as "[Hq5 Hq]".
+    iClear "Hq".
+    replace (q +ₗ 1 +ₗ 1) with (q +ₗ 2) in * by (rewrite Loc.add_assoc; done).
+    replace (q +ₗ 2 +ₗ 1) with (q +ₗ 3) in * by (rewrite Loc.add_assoc; done).
+    replace (q +ₗ 3 +ₗ 1) with (q +ₗ 4) in * by (rewrite Loc.add_assoc; done).
+    replace (q +ₗ 4 +ₗ 1) with (q +ₗ 5) in * by (rewrite Loc.add_assoc; done).
+    wp_alloc block as "Hblock".
+    { unfold BLOCK_ALLOC_SIZE, CHUNKED_QUEUE_BLOCK_SIZE. lia. }
+    wp_pures.
+    change (Z.to_nat BLOCK_ALLOC_SIZE) with 130%nat.
+    iDestruct (array_cons with "Hblock") as "[Hb0 Hblock]".
+    iDestruct (array_cons with "Hblock") as "[Hb1 Hblock]".
+    rewrite Loc.add_0. wp_store. wp_pures.
+    wp_store. wp_pures. wp_store. wp_pures. wp_store. wp_pures.
+    wp_store. wp_pures. wp_store. wp_pures. wp_store.
+    replace (block +ₗ 1 +ₗ 1) with (block +ₗ 2) in * by (rewrite Loc.add_assoc; done).
+    iMod (own_alloc (●ML{# (1/2)%Qp} ([] : list (leibnizO val)) ⋅ ●ML{# (1/2)%Qp} ([] : list (leibnizO val)))) as (γ_list) "[Hauth1 Hauth2]".
+    { rewrite -mono_list_auth_dfrac_op. rewrite dfrac_op_own Qp.half_half. apply mono_list_auth_valid. }
+    iMod (own_alloc (●ML{# 1%Qp} ([block] : list (leibnizO loc)))) as (γ_blocks) "Hblk_auth".
+    { apply mono_list_auth_valid. }
+    iMod (mono_nat_own_alloc 0) as (γ_head) "[Hhead_auth _]".
+    iMod (mono_nat_own_alloc 0) as (γ_tail) "[Htail_auth _]".
+    iMod (ghost_map_alloc_empty) as (γ_claims) "Hclaims".
+    iDestruct "Hhead_auth" as "[Hhead1 Hhead2]".
+    iDestruct "Htail_auth" as "[Htail1 Htail2]".
+    set (γ := QueueName γ_list γ_blocks γ_head γ_tail γ_claims).
+    iApply ("HΦ" $! γ). iSplitR "Hauth2 Hhead2 Htail2".
+    2:{ unfold queue_content. simpl. iFrame. iModIntro. done. }
+    iApply inv_alloc. iNext. unfold queue_inv_inner.
+    iExists [], 0%nat, 0%nat, 0%Z, block, block, CHUNKED_QUEUE_BLOCK_SIZE, [(block, 0%Z)], 0%nat, 0%nat, ∅.
+    simpl. iFrame "Hauth1 Hblk_auth Hhead1 Htail1 Hclaims".
+    rewrite Loc.add_0. iFrame "Hq0 Hq1 Hq2 Hq3 Hq4 Hq5".
+    iSplit; first done.
+    iSplit; first (iPureIntro; lia).
+    iSplit; first (iPureIntro; left; done).
+    iSplit; first done.
+    iSplit; first (iPureIntro; unfold CHUNKED_QUEUE_BLOCK_SIZE; lia).
+    iSplit; first (iPureIntro; reflexivity).
+    iSplit; first (iPureIntro; reflexivity).
+    iSplit; first (iPureIntro; intros i blk Hi; destruct i as [|[|]]; simpl in Hi; [inversion Hi; done|discriminate|discriminate]).
+    iSplit; first (iPureIntro; intros k _; apply lookup_empty).
+    unfold is_block_chain. simpl. unfold is_block. rewrite Loc.add_0. iFrame "Hb0 Hb1".
+    change BS with 64%nat. change (Z.to_nat 0) with 0%nat.
+    iAssert (∀ (n : nat), ⌜(n ≤ 64)%nat⌝ -∗
+      (block +ₗ (2 + 2 * Z.of_nat (64 - n))) ↦∗ replicate (2 * n) #0 -∗
+      [∗ list] i ∈ seq (64 - n) n, slot_inv γ_claims [] (0 * 64 + i)%nat (block +ₗ (2 + 2 * Z.of_nat i)))%I as "Hind".
+    { iIntros (n).
+      iInduction n as [|n'] "IH".
+      - iIntros "% Hblock". done.
+      - iIntros (Hn) "Hblock".
+        replace (64 - S n')%nat with (64 - n' - 1)%nat by lia.
+        replace (2 * S n')%nat with (2 + 2 * n')%nat by lia.
+        rewrite replicate_add.
+        iDestruct (array_app with "Hblock") as "[Hpair Hrest]".
+        simpl.
+        iDestruct (array_cons with "Hpair") as "[Hval Hpair]".
+        iDestruct (array_cons with "Hpair") as "[Hstate _]".
+        iSplitL "Hval Hstate".
+        { unfold slot_inv. iExists 0.
+          replace (block +ₗ (2 + 2 * (64 - n' - 1)%nat) +ₗ 1) with (block +ₗ (2 + 2 * Z.of_nat (64 - n' - 1)) +ₗ 1) by (f_equal; lia).
+          iFrame "Hstate". iLeft. iSplit; [done|]. iExists #0. iExact "Hval". }
+        replace (S (64 - n' - 1)) with (64 - n')%nat by lia.
+        iApply ("IH" with "[%] [Hrest]").
+        { lia. }
+        replace (block +ₗ (2 + 2 * (64 - n' - 1)%nat) +ₗ 2%nat) with (block +ₗ (2 + 2 * Z.of_nat (64 - n'))) by (rewrite Loc.add_assoc; f_equal; lia).
+        replace (n' + (n' + 0))%nat with (2 * n')%nat by lia.
+        done. }
+    iSpecialize ("Hind" $! 64%nat with "[%] [Hblock]").
+    { lia. }
+    { change (2 + 2 * Z.of_nat (64 - 64))%Z with 2%Z. done. }
+    replace (64 - 64)%nat with 0%nat by lia. done.
+  Defined.
 
   (** @spec: logically atomic push that appends data to L.
       @linpoint: FAA on queue.tail_idx. *)
@@ -311,7 +402,124 @@ Section spec.
     <<{ ∀∀ (L : list val) (h : nat), queue_content γ L h }>>
       chunked_queue_push #q v @ ↑queueN
     <<{ queue_content γ (L ++ [v]) h | RET #() }>>.
-  Proof. Admitted.
+  Proof.
+    iIntros "#Hinv" (Φ) "AU".
+    unfold chunked_queue_push. wp_pures.
+    (* === FAA linearization point === *)
+    wp_bind (FAA _ _).
+    iInv "Hinv" as (L h t lock_val hb tb cap blocks hi ti C)
+      ">(Hauth & Hblk_auth & Hhead & Htail & Hclaims & %Ht & %Hht & Hlock & %Hlock_val &
+         Hhb & Hh & Htb & Htail_loc & Hcap &
+         %Hblocks_ne & %Hcap_eq & %Hhi & %Hti & %Hbids & %Hcfresh & Hchain)".
+    wp_faa.
+    (* Open AU, agree on ghost state *)
+    iMod "AU" as (L' h') "[Hcontent [_ Hclose]]".
+    unfold queue_content.
+    iDestruct "Hcontent" as "(Hauth2 & Hhead2 & Htail2)".
+    iCombine "Hauth" "Hauth2" as "Hauth_full".
+    iDestruct (own_valid with "Hauth_full") as %Hvalid.
+    rewrite mono_list_auth_dfrac_op_valid in Hvalid.
+    destruct Hvalid as [_ HL]. apply leibniz_equiv in HL. subst L'.
+    iDestruct (mono_nat_auth_own_agree with "Hhead Hhead2") as %[_ Hheq].
+    subst h'.
+    iDestruct (mono_nat_auth_own_agree with "Htail Htail2") as %[_ Htlen].
+    (* Update mono_list: L → L ++ [v] *)
+    iMod (own_update with "Hauth_full") as "Hauth_full".
+    { rewrite -mono_list_auth_dfrac_op dfrac_op_own Qp.half_half.
+      apply (mono_list_update (L ++ [v])). apply prefix_app_r. done. }
+    iDestruct "Hauth_full" as "[Hauth1 Hauth2]".
+    (* Update mono_nat tail: length L → length (L ++ [v]) *)
+    iCombine "Htail" "Htail2" as "Htail". rewrite Htlen.
+    iDestruct "Htail" as "[Htail Htail2]".
+    iCombine "Htail" "Htail2" as "Htail".
+    iMod (mono_nat_own_update (length (L ++ [v])) with "Htail")
+      as "[[Htail Htail2] _]".
+    { rewrite app_length. simpl. lia. }
+    (* Close AU *)
+    iMod ("Hclose" with "[Hauth2 Hhead2 Htail2]") as "HΦ".
+    { iFrame. }
+    (* Close invariant *)
+    iSplitR "HΦ".
+    { iModIntro. iNext. unfold queue_inv_inner.
+      iExists (L ++ [v]), h, (length L + 1)%nat, lock_val, hb, tb,
+        cap, blocks, hi, ti, C.
+      replace (length L + 1)%Z with (Z.of_nat (length L + 1)%nat) in *
+        by lia.
+      rewrite app_length. simpl.
+      iFrame "Hauth1 Hblk_auth Hhead Htail Hclaims Hlock Hhb Hh Htb Htail_loc Hcap".
+      repeat iSplit; try (iPureIntro; first [done | lia]).
+      destruct blocks as [|[first bid] blocks']; first done.
+      iApply (big_sepL_mono with "Hchain").
+      iIntros (k [b bid'] Hlookup) "Hblock".
+      unfold is_block. iDestruct "Hblock" as "(Hnext & Hbid & Hslots)".
+      iFrame "Hnext Hbid".
+      iApply (big_sepL_mono with "Hslots").
+      iIntros (i x Hlookup2) "Hslot".
+      unfold slot_inv. iDestruct "Hslot" as (state) "[Hstate Hcases]".
+      iExists state. iFrame "Hstate".
+      iDestruct "Hcases" as "[H | [H | [H | H]]]".
+      - iLeft. done.
+      - iRight. iLeft. done.
+      - iRight. iRight. iLeft.
+        iDestruct "H" as "[%Hs2 H]". iSplit; first done.
+        iDestruct "H" as (w0) "[Hval %HLw]".
+        iExists w0. iFrame "Hval".
+        iPureIntro. apply lookup_app_l_Some. done.
+      - iRight. iRight. iRight. done. }
+    (* === Continuation: grow + find_block + slot writes === *)
+    iModIntro. wp_pures.
+    admit.
+  Admitted.
+
+  (* Helper: the find_slot_loop finds the block with the target block_id,
+     waits for the slot to become Valid, reads the value, resets state to Empty,
+     and returns the value. *)
+  Lemma find_slot_loop_spec γ (q : loc) (h1 : nat)
+      (L3 : list val) (blocks3 : list (loc * Z)) (d : val)
+      (Hlookup : L3 !! h1 = Some d) :
+    {{{ is_queue γ q ∗
+        own γ.(γ_list) (◯ML (L3 : list (leibnizO val))) ∗
+        own γ.(γ_blocks) (◯ML (blocks3.*1 : list (leibnizO loc))) ∗
+        h1 ↪[γ.(γ_claims)] () }}}
+      chunked_queue_pop_find_slot_loop #q
+         #(Z.quot (Z.of_nat h1) CHUNKED_QUEUE_BLOCK_SIZE)
+         #(Z.rem (Z.of_nat h1) CHUNKED_QUEUE_BLOCK_SIZE)
+    {{{ RET d; True }}}.
+  Proof.
+    iIntros (Φ) "(#Hinv & #Hlb_L & #Hlb_blocks & Hclaim) HΦ".
+    unfold chunked_queue_pop_find_slot_loop.
+    iLöb as "IH".
+    wp_rec. wp_pures.
+    (* Load cursor = !(queue +ₗ 1) = head_block *)
+    wp_bind (! _)%E.
+    iInv "Hinv" as (Lf hf tf lvf hbf tbf capf blocksf hif tif Cf)
+      ">(Haf & Hbaf & Hhf & Htf & Hclaimsf & %Htf_eq & %Hhtf & Hlkf & %Hlvf &
+         Hhbf & Hhfl & Htbf & Htfl & Hcapf &
+         %Hnef & %Hcef & %Hhif & %Htif & %Hbidsf & %Hcfreshf & Hchf)".
+    wp_load.
+    (* Save persistent fragment for current blocks *)
+    iDestruct (own_mono _ _ (◯ML (blocksf.*1 : list (leibnizO loc))) with "Hbaf") as "#Hlb_blocksf".
+    { apply mono_list_included. }
+    iModIntro. iSplitR "HΦ Hclaim".
+    { iNext. unfold queue_inv_inner.
+      iExists Lf, hf, tf, lvf, hbf, tbf, capf, blocksf, hif, tif, Cf.
+      iFrame. done. }
+    wp_pures.
+    (* Now call find_slot on the chain starting from hbf.
+       The inner find_slot walks the chain and eventually finds the block
+       with block_id = h1 / BS. We need to know hbf is in the chain.
+       From Hhif: blocksf !! hif = Some (hbf, hif). *)
+    (* We know hbf is at index hif in blocksf, and we have ◯ML blocksf.*1.
+       The target block_id = h1 quot BS. We need the block at that index
+       to exist in the chain. *)
+    set (block_id := Z.quot (Z.of_nat h1) CHUNKED_QUEUE_BLOCK_SIZE).
+    set (slot_idx := Z.rem (Z.of_nat h1) CHUNKED_QUEUE_BLOCK_SIZE).
+    (* The inner find_slot either finds the block and returns SOME d
+       (consuming the claim), or returns NONE (preserving the claim).
+       Proof of the inner call is admitted here. *)
+    wp_bind (chunked_queue_pop_find_slot _ _ _ _)%E.
+    admit.
+  Admitted.
 
   (** @spec: logically atomic pop that removes head from L.
       @linpoint: CAS on queue.head_idx. *)
@@ -327,6 +535,295 @@ Section spec.
           ⌜w = InjLV #()⌝ ∗ ⌜h = length L⌝ ∗
           queue_content γ L h)
       | RET (w, #ok)%V }>>.
-  Proof. Admitted.
+  Proof.
+    iIntros "#Hinv" (Φ) "AU".
+    unfold chunked_queue_pop. wp_pures.
+    wp_bind (chunked_queue_pop_cas_loop _)%E.
+    unfold chunked_queue_pop_cas_loop.
+    iLöb as "IH".
+    wp_rec. wp_pures.
+    (* Load head_idx *)
+    wp_bind (! _)%E.
+    iInv "Hinv" as (L1 h1 t1 lv1 hb1 tb1 cap1 blocks1 hi1 ti1 C1)
+      ">(Ha1 & Hba1 & Hh1 & Ht1 & Hclaims1 & %Ht1 & %Hht1 & Hlk1 & %Hlv1 &
+         Hhb1 & Hh1l & Htb1 & Htl1 & Hcap1 &
+         %Hne1 & %Hce1 & %Hhi1 & %Hti1 & %Hbids1 & %Hcfresh1 & Hch1)".
+    wp_load.
+    iDestruct (mono_nat_lb_own_get with "Hh1") as "#Hlb_h1".
+    iModIntro. iSplitR "AU".
+    { iNext. unfold queue_inv_inner.
+      iExists L1, h1, t1, lv1, hb1, tb1, cap1, blocks1, hi1, ti1, C1.
+      iFrame. done. }
+    wp_pures.
+    (* Load tail_idx *)
+    wp_bind (! _)%E.
+    iInv "Hinv" as (L2 h2 t2 lv2 hb2 tb2 cap2 blocks2 hi2 ti2 C2)
+      ">(Ha2 & Hba2 & Hh2 & Ht2 & Hclaims2 & %Ht2 & %Hht2 & Hlk2 & %Hlv2 &
+         Hhb2 & Hh2l & Htb2 & Htl2 & Hcap2 &
+         %Hne2 & %Hce2 & %Hhi2 & %Hti2 & %Hbids2 & %Hcfresh2 & Hch2)".
+    wp_load.
+    iDestruct (mono_nat_lb_own_valid with "Hh2 Hlb_h1") as %[_ Hh1_le_h2].
+    iDestruct (mono_nat_lb_own_get with "Ht2") as "#Hlb_t2".
+    destruct (decide (Z.of_nat t2 ≤ Z.of_nat h1)%Z) as [Hdec|Hdec].
+    + (* Empty case: t2 ≤ h1, so h2 = t2 = h1 = length L2 *)
+      assert (h2 = t2) as -> by lia.
+      assert (t2 = h1) as -> by lia.
+      iMod "AU" as (L' h') "[Hcontent [_ Hclose]]".
+      unfold queue_content.
+      iDestruct "Hcontent" as "(Hauth' & Hhead' & Htail')".
+      iCombine "Ha2" "Hauth'" as "Hauth_full".
+      iDestruct (own_valid with "Hauth_full") as %Hvalid.
+      rewrite mono_list_auth_dfrac_op_valid in Hvalid.
+      destruct Hvalid as [_ HLeq]. apply leibniz_equiv in HLeq. subst L'.
+      iDestruct "Hauth_full" as "[Ha2 Hauth']".
+      iDestruct (mono_nat_auth_own_agree with "Hh2 Hhead'") as %[_ Hheq]. subst h'.
+      iDestruct (mono_nat_auth_own_agree with "Ht2 Htail'") as %[_ Htleq].
+      iMod ("Hclose" $! (InjLV #()) false with "[Hauth' Hhead' Htail']") as "HΦ".
+      { iRight. iSplit; first done. iSplit; first done. iSplit.
+        - iPureIntro. lia.
+        - unfold queue_content. iFrame. }
+      iModIntro. iSplitR "HΦ".
+      { iNext. unfold queue_inv_inner.
+        iExists L2, h1, h1, lv2, hb2, tb2, cap2, blocks2, hi2, ti2, C2.
+        iFrame. done. }
+      wp_pures.
+      rewrite bool_decide_eq_true_2; last lia.
+      wp_pures. done.
+    + (* Non-empty case: h1 < t2 *)
+      iModIntro. iSplitR "AU".
+      { iNext. unfold queue_inv_inner.
+        iExists L2, h2, t2, lv2, hb2, tb2, cap2, blocks2, hi2, ti2, C2.
+        iFrame. done. }
+      wp_pures.
+      rewrite bool_decide_eq_false_2; last lia.
+      wp_pures.
+      (* CAS on head_idx *)
+      wp_bind (CmpXchg _ _ _).
+      iInv "Hinv" as (L3 h3 t3 lv3 hb3 tb3 cap3 blocks3 hi3 ti3 C3)
+        ">(Ha3 & Hba3 & Hh3 & Ht3 & Hclaims3 & %Ht3 & %Hht3 & Hlk3 & %Hlv3 &
+           Hhb3 & Hh3l & Htb3 & Htl3 & Hcap3 &
+           %Hne3 & %Hce3 & %Hhi3 & %Hti3 & %Hbids3 & %Hcfresh3 & Hch3)".
+      destruct (decide (h3 = h1)) as [->|Hne].
+      - (* CAS success *)
+        wp_cmpxchg_suc.
+        iMod "AU" as (L' h') "[Hcontent [_ Hclose]]".
+        unfold queue_content.
+        iDestruct "Hcontent" as "(Hauth' & Hhead' & Htail')".
+        iCombine "Ha3" "Hauth'" as "Hauth_full".
+        iDestruct (own_valid with "Hauth_full") as %Hvalid.
+        rewrite mono_list_auth_dfrac_op_valid in Hvalid.
+        destruct Hvalid as [_ HLeq]. apply leibniz_equiv in HLeq. subst L'.
+        iDestruct "Hauth_full" as "[Ha3 Hauth']".
+        iDestruct (mono_nat_auth_own_agree with "Hh3 Hhead'") as %[_ Hheq]. subst h'.
+        iDestruct (mono_nat_auth_own_agree with "Ht3 Htail'") as %[_ Htleq].
+        iDestruct (mono_nat_lb_own_valid with "Ht3 Hlb_t2") as %[_ Ht2_le_t3].
+        assert (h1 < t3) as Hh1_lt_t3 by lia.
+        assert (h1 < length L3) as Hh1_lt_len by lia.
+        destruct (L3 !! h1) as [d|] eqn:Hlookup;
+          last by (exfalso; apply lookup_ge_None in Hlookup; lia).
+        iCombine "Hh3" "Hhead'" as "Hhead_full".
+        iMod (mono_nat_own_update (S h1) with "Hhead_full") as "[[Hh3 Hhead'] _]".
+        { lia. }
+        (* Persistent lower bounds for continuation proofs *)
+        iDestruct (own_mono _ _ (◯ML (L3 : list (leibnizO val))) with "Ha3") as "#Hlb_L3".
+        { apply mono_list_included. }
+        iDestruct (own_mono _ _ (◯ML (blocks3.*1 : list (leibnizO loc))) with "Hba3") as "#Hlb_blocks3".
+        { apply mono_list_included. }
+        (* Allocate consumer claim token *)
+        iMod (ghost_map_insert h1 () with "Hclaims3") as "[Hclaims3 Hclaim]".
+        { apply Hcfresh3. lia. }
+        iMod ("Hclose" $! (InjRV d) true with "[Hauth' Hhead' Htail']") as "HΦ".
+        { iLeft. iSplit; first done. iExists d. iSplit; first done. iSplit; first done.
+          unfold queue_content. iFrame. }
+        replace (h1 + 1)%Z with (Z.of_nat (S h1)) by lia.
+        iModIntro. iSplitR "HΦ Hclaim".
+        { iNext. unfold queue_inv_inner.
+          iExists L3, (S h1), t3, lv3, hb3, tb3, cap3, blocks3, hi3, ti3, (<[h1 := ()]> C3).
+          iFrame. iPureIntro. repeat split; try done; try lia.
+          intros k Hk. rewrite lookup_insert_ne; [apply Hcfresh3; lia | lia]. }
+        wp_pures.
+        (* Continuation: advance_head_loop + find_slot_loop *)
+        destruct (bool_decide (#(h1 `rem` CHUNKED_QUEUE_BLOCK_SIZE) = #0)) eqn:Hrem_dec.
+        ** (* slot_idx = 0 *)
+           wp_pures.
+           destruct (decide (0 < h1)%nat) as [Hh1_pos|Hh1_zero].
+           --- (* h1 > 0 && slot_idx = 0: advance_head_loop needed *)
+               rewrite bool_decide_eq_true_2; last lia.
+               wp_pures.
+               wp_bind (chunked_queue_pop_advance_head_loop _ _).
+               unfold chunked_queue_pop_advance_head_loop.
+               iLöb as "IH_adv".
+               wp_rec. wp_pures.
+               (* Load old_head = queue.head_block *)
+               wp_bind (! _)%E.
+               iInv "Hinv" as (La ha ta lva hba tba capa blocksa hia tia Ca)
+                 ">(Haa & Hbaa & Hha & Hta & Hclaimsa & %Hta_eq & %Hhta & Hlka & %Hlva &
+                    Hhba & Hhla & Htba & Htla & Hcapa &
+                    %Hnea & %Hcea & %Hhia & %Htia & %Hbidsa & %Hcfresha & Hcha)".
+               wp_load.
+               (* Save persistent lower bound for blocksa *)
+               iDestruct (own_mono _ _ (◯ML (blocksa.*1 : list (leibnizO loc))) with "Hbaa") as "#Hlb_blocksa".
+               { apply mono_list_included. }
+               iModIntro. iSplitR "IH_adv HΦ Hclaim".
+               { iNext. unfold queue_inv_inner.
+                 iExists La, ha, ta, lva, hba, tba, capa, blocksa, hia, tia, Ca.
+                 iFrame. done. }
+               wp_pures.
+               (* Now need to read hba.block_id — open invariant again *)
+               wp_bind (! _)%E.
+               iInv "Hinv" as (Lb hb0 tb0 lvb hbb tbb capb blocksb hib tib Cb)
+                 ">(Hab & Hbab & Hhb & Htb & Hclaimsb & %Htb_eq & %Hhtb & Hlkb & %Hlvb &
+                    Hhbb & Hhlb & Htbb & Htlb & Hcapb &
+                    %Hneb & %Hceb & %Hhib & %Htib & %Hbidsb & %Hcfreshb & Hchb)".
+               (* Prove hba is in current blocks via prefix *)
+               iDestruct (own_valid_2 with "Hbab Hlb_blocksa") as %Hpfx_ab.
+               rewrite mono_list_both_dfrac_valid_L in Hpfx_ab.
+               destruct Hpfx_ab as [_ Hpfx_ab].
+               assert (hia < length blocksa) as Hhia_lt by (eapply lookup_lt_Some; eauto).
+               assert (hia < length blocksb) as Hhia_lt_b.
+               { apply prefix_length in Hpfx_ab. rewrite !length_fmap in Hpfx_ab. lia. }
+               assert (blocksa.*1 !! hia = Some hba) as Hhba_in_a.
+               { rewrite list_lookup_fmap. rewrite Hhia. done. }
+               assert (blocksb.*1 !! hia = Some hba) as Hhba_in_b.
+               { eapply prefix_lookup_Some; eauto. }
+               assert (∃ bid_b, blocksb !! hia = Some (hba, bid_b)) as [bid_b Hhba_blk_b].
+               { rewrite list_lookup_fmap in Hhba_in_b.
+                 destruct (blocksb !! hia) as [[lb bidb]|] eqn:Hlb; [|discriminate].
+                 simpl in Hhba_in_b. inversion Hhba_in_b. subst. eauto. }
+               assert (bid_b = Z.of_nat hia) as -> by (apply (Hbidsb _ _ Hhba_blk_b)).
+               destruct blocksb as [|[firstb firstbid] blocksb']; first done.
+               iDestruct (big_sepL_lookup_acc with "Hchb") as "[Hblk Hchb_rest]"; first exact Hhba_blk_b.
+               unfold is_block.
+               iDestruct "Hblk" as "(Hnext_b & Hbid_b & Hslots_b)".
+               wp_load.
+               iDestruct ("Hchb_rest" with "[Hnext_b Hbid_b Hslots_b]") as "Hchb".
+               { unfold is_block. iFrame. }
+               iModIntro. iSplitR "IH_adv HΦ Hclaim".
+               { iNext. unfold queue_inv_inner.
+                 iExists Lb, hb0, tb0, lvb, hbb, tbb, capb, ((firstb, firstbid) :: blocksb'), hib, tib, Cb.
+                 iFrame. done. }
+               wp_pures.
+               (* block_id ≤ hia? *)
+               destruct (decide (Z.quot (Z.of_nat h1) CHUNKED_QUEUE_BLOCK_SIZE ≤ Z.of_nat hia)%Z) as [Hbd_le|Hbd_gt].
+               +++ (* block_id ≤ hia: loop done *)
+                   rewrite bool_decide_eq_true_2; last done.
+                   wp_pures.
+                   wp_apply (find_slot_loop_spec with "[$Hinv $Hlb_L3 $Hlb_blocks3 $Hclaim]"); [done|].
+                   iIntros "_". wp_pures. done.
+               +++ (* block_id > hia: need to advance, read next, CAS, loop *)
+                   rewrite bool_decide_eq_false_2; last done.
+                   wp_pures.
+                   (* Read next pointer from hba *)
+                   wp_bind (! _)%E.
+                   iInv "Hinv" as (Lc hc tc lvc hbc tbc capc blocksc hic tic Cc)
+                     ">(Hac & Hbac & Hhc & Htc & Hclaimsc & %Htc_eq & %Hhtc & Hlkc & %Hlvc &
+                        Hhbc & Hhlc & Htbc & Htlc & Hcapc &
+                        %Hnec & %Hcec & %Hhic & %Htic & %Hbidsc & %Hcfreshc & Hchc)".
+                   iDestruct (own_valid_2 with "Hbac Hlb_blocksa") as %Hpfx_ac.
+                   rewrite mono_list_both_dfrac_valid_L in Hpfx_ac.
+                   destruct Hpfx_ac as [_ Hpfx_ac].
+                   assert (hia < length blocksc) as Hhia_lt_c.
+                   { apply prefix_length in Hpfx_ac. rewrite !length_fmap in Hpfx_ac. lia. }
+                   assert (blocksc.*1 !! hia = Some hba) as Hhba_in_c.
+                   { eapply prefix_lookup_Some. exact Hhba_in_a. exact Hpfx_ac. }
+                   assert (∃ bid_c, blocksc !! hia = Some (hba, bid_c)) as [bid_c Hhba_blk_c].
+                   { rewrite list_lookup_fmap in Hhba_in_c.
+                     destruct (blocksc !! hia) as [[lc bidc]|] eqn:Hlc; [|discriminate].
+                     simpl in Hhba_in_c. inversion Hhba_in_c. subst. eauto. }
+                   assert (bid_c = Z.of_nat hia) as -> by (apply (Hbidsc _ _ Hhba_blk_c)).
+                   (* Save persistent lb for blocksc before destructing *)
+                   iDestruct (own_mono _ _ (◯ML (blocksc.*1 : list (leibnizO loc))) with "Hbac") as "#Hlb_blocksc".
+                   { apply mono_list_included. }
+                   destruct blocksc as [|[firstc firstcidb] blocksc']; first done.
+                   iDestruct (big_sepL_lookup_acc with "Hchc") as "[Hblk_c Hchc_rest]"; first exact Hhba_blk_c.
+                   unfold is_block.
+                   iDestruct "Hblk_c" as "(Hnext_c & Hbid_c & Hslots_c)".
+                   wp_load.
+                   iDestruct ("Hchc_rest" with "[Hnext_c Hbid_c Hslots_c]") as "Hchc".
+                   { unfold is_block. iFrame. }
+                   iModIntro. iSplitR "IH_adv HΦ Hclaim".
+                   { iNext. unfold queue_inv_inner.
+                     iExists Lc, hc, tc, lvc, hbc, tbc, capc, ((firstc, firstcidb) :: blocksc'), hic, tic, Cc.
+                     iFrame. done. }
+                   wp_pures.
+                   (* CAS on queue.head_block *)
+                   wp_bind (CmpXchg _ _ _).
+                   iInv "Hinv" as (Ld hd td lvd hbd tbd capd blocksd hid tid Cd)
+                     ">(Had & Hbad & Hhd & Htd & Hclaimsd & %Htd_eq & %Hhtd & Hlkd & %Hlvd &
+                        Hhbd & Hhld & Htbd & Htld & Hcapd &
+                        %Hned & %Hced & %Hhid & %Htid & %Hbidsd & %Hcfreshd & Hchd)".
+                   destruct (decide (hbd = hba)) as [->|Hne_hbd].
+                   *** (* CAS success: head_block = hba, update to next *)
+                       wp_cmpxchg_suc.
+                       (* blocksc.*1 prefix of blocksd.*1 *)
+                       iDestruct (own_valid_2 with "Hbad Hlb_blocksc") as %Hpfx_cd.
+                       rewrite mono_list_both_dfrac_valid_L in Hpfx_cd.
+                       destruct Hpfx_cd as [_ Hpfx_cd].
+                       (* block_next case split: S hia within blocksc or wraps to firstc *)
+                       set (bnext := block_next ((firstc, firstcidb) :: blocksc') hia firstc).
+                       destruct (((firstc, firstcidb) :: blocksc') !! (S hia)) as [[next_loc next_bid]|] eqn:Hnext_blk.
+                       ---- (* S hia within blocksc: next = block at S hia *)
+                         assert (bnext = next_loc) as Hbn.
+                         { unfold bnext, block_next. rewrite Hnext_blk. done. }
+                         assert (((firstc, firstcidb) :: blocksc').*1 !! (S hia) = Some next_loc) as Hnext_in_c.
+                         { rewrite list_lookup_fmap. rewrite Hnext_blk. done. }
+                         assert (blocksd.*1 !! (S hia) = Some next_loc) as Hnext_in_d.
+                         { eapply prefix_lookup_Some; eauto. }
+                         assert (∃ bid_d, blocksd !! (S hia) = Some (next_loc, bid_d)) as [bid_d2 Hnext_blk_d].
+                         { rewrite list_lookup_fmap in Hnext_in_d.
+                           destruct (blocksd !! S hia) as [[ld bidd]|] eqn:Hsd; [|discriminate].
+                           simpl in Hnext_in_d. injection Hnext_in_d as <-. eauto. }
+                         assert (bid_d2 = Z.of_nat (S hia)) as -> by (apply (Hbidsd _ _ Hnext_blk_d)).
+                         rewrite Hbn.
+                         iModIntro. iSplitR "IH_adv HΦ Hclaim".
+                         { iNext. unfold queue_inv_inner.
+                           iExists Ld, hd, td, lvd, next_loc, tbd, capd, blocksd, (S hia), tid, Cd.
+                           iFrame. iPureIntro. repeat split; try done; try lia. }
+                         wp_proj. wp_seq.
+                         iApply ("IH_adv" with "HΦ Hclaim").
+                       ---- (* S hia out of bounds: next wraps to firstc = block 0 *)
+                         assert (bnext = firstc) as Hbn.
+                         { unfold bnext, block_next. rewrite Hnext_blk. done. }
+                         assert (blocksd.*1 !! 0 = Some firstc) as Hfirst_in_d.
+                         { eapply prefix_lookup_Some; last exact Hpfx_cd.
+                           done. }
+                         assert (∃ bid_d, blocksd !! 0 = Some (firstc, bid_d)) as [bid_d2 Hfirst_blk_d].
+                         { rewrite list_lookup_fmap in Hfirst_in_d.
+                           destruct (blocksd !! 0) as [[ld bidd]|] eqn:Hsd; [|discriminate].
+                           simpl in Hfirst_in_d. injection Hfirst_in_d as <-. eauto. }
+                         assert (bid_d2 = Z.of_nat 0) as -> by (apply (Hbidsd _ _ Hfirst_blk_d)).
+                         rewrite Hbn.
+                         iModIntro. iSplitR "IH_adv HΦ Hclaim".
+                         { iNext. unfold queue_inv_inner.
+                           iExists Ld, hd, td, lvd, firstc, tbd, capd, blocksd, 0%nat, tid, Cd.
+                           iFrame. iPureIntro. repeat split; try done; try lia. }
+                         wp_proj. wp_seq.
+                         iApply ("IH_adv" with "HΦ Hclaim").
+                   *** (* CAS fail: head_block ≠ hba *)
+                       wp_cmpxchg_fail.
+                       iModIntro. iSplitR "IH_adv HΦ Hclaim".
+                       { iNext. unfold queue_inv_inner.
+                         iExists Ld, hd, td, lvd, hbd, tbd, capd, blocksd, hid, tid, Cd.
+                         iFrame. done. }
+                       wp_proj. wp_seq.
+                       iApply ("IH_adv" with "HΦ Hclaim").
+           --- (* h1 = 0: no advance needed *)
+               assert (h1 = 0) as -> by lia.
+               rewrite bool_decide_eq_false_2; last lia.
+               wp_pures.
+               wp_apply (find_slot_loop_spec with "[$Hinv $Hlb_L3 $Hlb_blocks3 $Hclaim]"); [done|].
+               iIntros "_". wp_pures. done.
+        ** (* slot_idx ≠ 0 case - no advance_head_loop *)
+           wp_pures.
+           wp_apply (find_slot_loop_spec with "[$Hinv $Hlb_L3 $Hlb_blocks3 $Hclaim]"); [done|].
+           iIntros "_". wp_pures. done.
+      - (* CAS fail *)
+        wp_cmpxchg_fail. { intros H. inversion H. lia. }
+        iModIntro. iSplitR "AU".
+        { iNext. unfold queue_inv_inner.
+          iExists L3, h3, t3, lv3, hb3, tb3, cap3, blocks3, hi3, ti3, C3.
+          iFrame. done. }
+        wp_proj. wp_if. iApply ("IH" with "AU").
+  Defined.
 
 End spec.
